printing program state

src/out/Test.ml
@@ -1,35 +1,75 @@
 open Prims
-let (bc1 : Structs.bytecode) =
-  Structs.CODE [Structs.LOAD_CONST Prims.int_one; Structs.RETURN_VALUE]
-let (co_test1 : Structs.codeObj) =
-  {
-    Structs.co_code = bc1;
-    Structs.co_consts =
-      [Structs.PYTYP (PyNone.createNone ());
-      Structs.PYTYP (PyInt.createInt (Prims.of_int (3)))];
-    Structs.co_varnames = [];
-    Structs.co_names = []
-  }
-let (bc2 : Structs.bytecode) =
+let (bc_0x7fefbe736660 : Structs.bytecode) =
+  Structs.CODE
+    [Structs.LOAD_CONST Prims.int_zero;
+    Structs.LOAD_CONST Prims.int_one;
+    Structs.MAKE_FUNCTION Prims.int_zero;
+    Structs.STORE_NAME Prims.int_zero;
+    Structs.LOAD_CONST (Prims.of_int (2));
+    Structs.LOAD_CONST (Prims.of_int (3));
+    Structs.MAKE_FUNCTION Prims.int_zero;
+    Structs.STORE_NAME Prims.int_one;
+    Structs.LOAD_CONST (Prims.of_int (4));
+    Structs.RETURN_VALUE]
+let (bc_0x7fefbe7365b0 : Structs.bytecode) =
   Structs.CODE
     [Structs.LOAD_CONST Prims.int_one;
     Structs.STORE_FAST Prims.int_zero;
-    Structs.LOAD_CONST (Prims.of_int (2));
-    Structs.STORE_FAST Prims.int_one;
     Structs.LOAD_FAST Prims.int_zero;
-    Structs.LOAD_FAST Prims.int_one;
-    Structs.BINARY_ADD;
-    Structs.STORE_FAST (Prims.of_int (2));
-    Structs.LOAD_FAST (Prims.of_int (2));
     Structs.RETURN_VALUE]
-let (co_test2 : Structs.codeObj) =
+let (consts_0x7fefbe7365b0 : Structs.pyObj Prims.list) =
+  [Structs.PYTYP (PyNone.createNone ());
+  Structs.PYTYP (PyInt.createInt (Prims.of_int (7)))]
+let (varnames_0x7fefbe7365b0 : Prims.string Prims.list) = ["y"]
+let names_0x7fefbe7365b0 : 'uuuuu . unit -> 'uuuuu Prims.list =
+  fun uu___ -> []
+let (co_0x7fefbe7365b0 : Structs.codeObj) =
   {
-    Structs.co_code = bc2;
-    Structs.co_consts =
-      [Structs.PYTYP (PyNone.createNone ());
-      Structs.PYTYP (PyInt.createInt Prims.int_one);
-      Structs.PYTYP (PyInt.createInt (Prims.of_int (2)))];
-    Structs.co_varnames = ["x"; "y"; "Z"];
-    Structs.co_names = []
+    Structs.co_code = bc_0x7fefbe7365b0;
+    Structs.co_consts = consts_0x7fefbe7365b0;
+    Structs.co_varnames = varnames_0x7fefbe7365b0;
+    Structs.co_names = (names_0x7fefbe7365b0 ())
   }
-let (res : Structs.pyObj) = VM.runCode co_test2
+let (bc_0x7fefbe736450 : Structs.bytecode) =
+  Structs.CODE
+    [Structs.LOAD_CONST Prims.int_one;
+    Structs.STORE_FAST Prims.int_zero;
+    Structs.LOAD_FAST Prims.int_zero;
+    Structs.RETURN_VALUE]
+let (consts_0x7fefbe736450 : Structs.pyObj Prims.list) =
+  [Structs.PYTYP (PyNone.createNone ());
+  Structs.PYTYP (PyInt.createInt (Prims.of_int (5)))]
+let (varnames_0x7fefbe736450 : Prims.string Prims.list) = ["x"]
+let names_0x7fefbe736450 : 'uuuuu . unit -> 'uuuuu Prims.list =
+  fun uu___ -> []
+let (co_0x7fefbe736450 : Structs.codeObj) =
+  {
+    Structs.co_code = bc_0x7fefbe736450;
+    Structs.co_consts = consts_0x7fefbe736450;
+    Structs.co_varnames = varnames_0x7fefbe736450;
+    Structs.co_names = (names_0x7fefbe736450 ())
+  }
+let (consts_0x7fefbe736660 : Structs.pyObj Prims.list) =
+  [Structs.CODEOBJECT co_0x7fefbe736450;
+  Structs.PYTYP (PyString.createString "first_function");
+  Structs.CODEOBJECT co_0x7fefbe7365b0;
+  Structs.PYTYP (PyString.createString "second_function");
+  Structs.PYTYP (PyNone.createNone ())]
+let varnames_0x7fefbe736660 : 'uuuuu . unit -> 'uuuuu Prims.list =
+  fun uu___ -> []
+let (names_0x7fefbe736660 : Prims.string Prims.list) =
+  ["first_function"; "second_function"]
+let (co_0x7fefbe736660 : Structs.codeObj) =
+  {
+    Structs.co_code = bc_0x7fefbe736660;
+    Structs.co_consts = consts_0x7fefbe736660;
+    Structs.co_varnames = (varnames_0x7fefbe736660 ());
+    Structs.co_names = names_0x7fefbe736660
+  }
+let (uu___0 : (Structs.vm * Structs.pyObj)) =
+  VM.runCode_returnVM co_0x7fefbe736660
+let (res : Structs.vm) = match uu___0 with | (res1, virt_m) -> res1
+let (virt_m : Structs.pyObj) = match uu___0 with | (res1, virt_m1) -> virt_m1
+let (print_program_state : unit) =
+  let uu___ = Utils.print_program_state res virt_m in
+  FStar_IO.print_string uu___
