test/autotest.py
@@ -43,26 +43,10 @@ if __name__=="__main__":
         t0 = time.time()
     
     result = subprocess.run([f'./{output_file}.exe'], stdout=subprocess.PIPE, 
-                            shell=True, cwd='/home/akarkour/pystar/PyStar/src/out')    
-    
-    if Config.PERFROMANCE_TEST:
-        t1 = time.time()
-        total_time = t1 - t0
-    
+                            shell=True, cwd='/home/akarkour/pystar/PyStar/src/out')
+    # print(result.stdout.decode("utf-8") )
     assert(result.returncode == 0)
-    
-    print(f'PY* RUN TIME ----> {total_time}')
-
-    # run code using another compiler
-    if Config.PERFROMANCE_TEST:
-        t0 = time.time()
-        
-    # exec(code_obj)
-    execute = os.system(f'python {input_file}')
-    if Config.PERFROMANCE_TEST:
-        t1 = time.time()
-        total_time = t1 - t0
-     
-    print(f'CPYTHON RUN TIME ----> {total_time}')
-    
+         
     # compare states
+    state_list = result.stdout.decode("utf-8").split("---\n")
+    print(state_list)
