src/VM.fsti
@@ -9,3 +9,4 @@ open Exec
 (* Takes in code object and execute it *)
 val runCode: codeObj -> All.ML pyObj
 
+val runCode_returnVM: codeObj -> All.ML (vm * pyObj)
